src/Set.v
@@ -1,20 +1,39 @@
 
 Class set(T E: Type) := mkSet {
+  contains: T -> E -> Prop;
+
   empty_set: T;
   singleton_set: E -> T;
+
   union: T -> T -> T;
   intersect: T -> T -> T;
   diff: T -> T -> T;
-  contains: T -> E -> Prop;
+
+  empty_set_spec: forall (x: E), contains empty_set x <-> False;
+  singleton_set_spec: forall (x y: E), contains (singleton_set y) x <-> x = y;
+  union_spec: forall (x: E) (A B: T), contains (union A B) x <-> contains A x \/ contains B x;
+  intersect_spec: forall (x: E) (A B: T), contains (intersect A B) x <-> contains A x /\ contains B x;
+  diff_spec: forall (x: E) (A B: T), contains (diff A B) x <-> contains A x /\ ~ contains B x
 }.
 
 Notation "x '\in' s" := (contains s x) (at level 39, no associativity).
 
+Section SetDefinitions.
+  Context {T E: Type}.
+  Context {setInst: set T E}.
+
+  Definition subset(s1 s2: T) := forall x, x \in s1 -> x \in s2.
+  Definition disjoint(s1 s2: T) := forall x, (~ x \in s1) \/ (~ x \in s2).
+
+End SetDefinitions.
+
 Instance Function_Set(E: Type): set (E -> Prop) E := {|
+  contains := fun s => s;
   empty_set := fun _ => False;
   singleton_set y := fun x => x = y;
   union := fun s1 s2 => fun x => s1 x \/ s2 x;
   intersect := fun s1 s2 => fun x => s1 x /\ s2 x;
-  diff := fun s1 s2 => fun x => s1 x /\ ~ s2 x;
-  contains := fun s => s
+  diff := fun s1 s2 => fun x => s1 x /\ ~ s2 x
 |}.
+  all: tauto.
+Defined.
